Factorize all the split_blocks functions

code/streaming/Hacl.Streaming.Interface.fsti
@@ -20,6 +20,7 @@ module U64 = FStar.UInt64
 
 open LowStar.BufferOps
 open FStar.Mul
+open Spec.Hash.Split
 
 inline_for_extraction noextract
 let uint8 = Lib.IntTypes.uint8
@@ -293,21 +294,14 @@ type block (index: Type0) =
     key: key.t i ->
     input:S.seq uint8 { S.length input <= max_input_length i } ->
     Lemma (
-      let open FStar.Mul in
-      let block_length = U32.v (block_len i) in
-      (**) Math.Lemmas.nat_over_pos_is_nat (S.length input) block_length;
-      (* TODO: factorize those 3 lines by using Spec.Hash.Incremental.split_blocks *)
-      let n = S.length input / block_length in
-      let rem = S.length input % block_length in (**)
-      let n, rem = if rem = 0 && n > 0 then n - 1, block_length else n, rem in (**)
-      (**) Math.Lemmas.nat_times_nat_is_nat n block_length;
-      let bs, l = S.split input (n * block_length) in
-      (**) Math.Lemmas.multiple_modulo_lemma n block_length;
+      let bs, l = gen_split_blocks (U32.v (block_len i)) input in
       (**) Math.Lemmas.modulo_lemma 0 (U32.v (block_len i));
       (* TODO: use update_full ? *)
-      let hash = update_multi_s i (init_s i key) 0 bs in
-      let hash = update_last_s i hash (n * block_length) l in
-      finish_s i key hash `S.equal` spec_s i key input)) -> (**)
+      let hash0 = init_s i key in
+      let hash1 = update_multi_s i hash0 0 bs in
+      let hash2 = update_last_s i hash1 (S.length bs) l in
+      let hash3 = finish_s i key hash2 in
+      hash3 `S.equal` spec_s i key input)) -> (**)
 
   // Stateful operations
   (* val *) index_of_state: (i:G.erased index -> (
